Add option methods

src/polycodable.lean
@@ -68,37 +68,24 @@ instance {α : Type} [polycodable α] : polycodable (option α) :=
   end  }
 
 def is_polytime {α β : Type} [polycodable α] [polycodable β] (f : α → β) : Prop :=
-∃ c : code, polytime c ∧ ∀ x : ℕ, c.eval x = part.some (encode ((decode α x).map f))
+∃ c : code, polytime c ∧ ∀ x, c.eval (encode x) = part.some (encode $ f x)
 
 @[simps] def polycodable.mk' {α : Type} (encode : α → ℕ) (decode : ℕ → option α) (decode_encode : ∀ x, decode (encode x) = some x)
   (poly : is_polytime (λ x, (decode x).map encode)) : polycodable α := 
 { encode := encode,
   decode := decode,
   decode_encode := decode_encode,
-  poly :=
-  begin
-    obtain ⟨c, pc, hc⟩ := poly,
-    use tail.comp c,
-    split, { exact polytime_comp polytime_tail pc, },
-    intro x, specialize hc x,
-    simp [hc, polycodable.encode],
-  end }
+  poly := by simpa [is_polytime, polycodable.encode] using poly }
 
 variables {α β γ : Type} [polycodable α] [polycodable β] [polycodable γ]
 
 lemma encode_decode_is_polytime : is_polytime (λ x : ℕ, (decode α x).map encode) :=
-begin
-  obtain ⟨c, pc, hc⟩ := poly α,
-  use (code.bit tt).comp c,
-  split, { exact polytime_comp (polytime_bit _) pc, },
-  intro x, specialize hc x,
-  simp [hc, polycodable.encode, nat.bit],
-end
+by simpa [is_polytime, polycodable.encode] using poly α
 
 lemma is_polytime_iff (f : α → β) :
-  is_polytime f ↔ ∃ c : code, polytime c ∧ ∀ x : α, c.eval (encode x) = part.some (encode (f x)) :=
+  is_polytime f ↔ ∃ c : code, polytime c ∧ ∀ x : ℕ, c.eval x = part.some (encode $ (decode α x).map f) :=
 begin
-  split,
+  split, swap,
   { rintro ⟨c, pc, hc⟩,
     use tail.comp c,
     split, { exact polytime_comp polytime_tail pc,},
@@ -113,43 +100,29 @@ begin
   { simp [hde], refl, }, simp [hde, hc], refl,
 end
 
-lemma is_polytime_comp {f : β → γ} {g : α → β} (hf : is_polytime f) (hg : is_polytime g) : is_polytime (f ∘ g) :=
-begin
-  simp only [is_polytime_iff] at *,
-  rcases hf with ⟨fc, pfc, hfc⟩, rcases hg with ⟨gc, pgc, hgc⟩,
-  use [fc.comp gc, polytime_comp pfc pgc], intro, simp [hfc, hgc],
-end
+lemma is_polytime_comp {f : β → γ} {g : α → β} : is_polytime f → is_polytime g → is_polytime (f ∘ g)
+| ⟨fc, fp, hf⟩ ⟨gc, gp, hg⟩ := ⟨fc.comp gc, polytime_comp fp gp, λ x, by simp [hf, hg]⟩
 
-lemma is_polytime_encode : is_polytime (@encode α _) :=
-by { rw is_polytime_iff, use [code.id, polytime_id], intro, simp, }
+lemma is_polytime_encode (α : Type) [polycodable α] : is_polytime (@encode α _) :=
+⟨code.id, polytime_id, λ x, by simp⟩
 
-lemma is_polytime_decode : is_polytime (decode α) :=
-by { rw is_polytime_iff, exact poly α, }
+lemma is_polytime_decode (α : Type) [polycodable α] : is_polytime (decode α) := poly α
 
-lemma is_polytime_option_elim (n : β) {s : α → β} (hs : is_polytime s) : is_polytime (λ x : option α, x.elim n s) :=
-begin
-  simp only [is_polytime_iff] at *,
-  rcases hs with ⟨sc, psc, hsc⟩,
-  use code.case zero sc (code.const (encode n)), split, { exact polytime_case polytime_zero psc (polytime_const _), },
-  intro x, cases x; simp [encode, hsc],
-end
+lemma is_polytime_const (β : Type) [polycodable β] (x : α) : is_polytime (λ _ : β, x) :=
+⟨code.const (encode x), polytime_const _, λ x, by simp⟩ 
 
-lemma is_polytime_some : is_polytime (@some α) :=
-by { rw is_polytime_iff, use code.bit tt, split, { exact polytime_bit _, }, simp [encode, nat.bit], }
+instance : polycodable bool :=
+polycodable.mk'
+(λ b, cond b 1 0) (λ n, some (if n = 0 then ff else tt)) (λ x, by cases x; simp)
+⟨(code.bit tt).comp to_bit, polytime_comp (polytime_bit _) polytime_to_bit, λ x, by cases x; simp; refl⟩
 
-lemma is_polytime_option_map {f : α → β} (hf : is_polytime f) : is_polytime (λ x : option α, x.map f) :=
-begin
-  convert_to is_polytime (λ x : option α, x.elim none (λ x', some (f x'))),
-  { ext x : 1, cases x; simp, },
-  exact is_polytime_option_elim _ (is_polytime_comp is_polytime_some hf),
-end
+lemma is_polytime_cond {c : α → bool} {f g : α → β} : is_polytime c → is_polytime f → is_polytime g → is_polytime (λ x, cond (c x) (f x) (g x))
+| ⟨cc, cp, hc⟩ ⟨fc, fp, hf⟩ ⟨gc, gp, hg⟩ :=
+⟨code.ite cc gc fc, (polytime_ite cp gp fp), λ x, by cases e : c x; simp [hc, hf, hg, e]⟩
 
-lemma is_polytime_option_bind {f : α → option β} (hf : is_polytime f) : is_polytime (λ x : option α, x.bind f) :=
-begin
-  convert_to is_polytime (λ x : option α, x.elim none (λ x', f x')),
-  { ext x : 1, cases x; simp, },
-  apply is_polytime_option_elim _ hf,
-end
+lemma is_polytime_is_some (α : Type) [polycodable α] : is_polytime (@option.is_some α) :=
+⟨to_bit, polytime_to_bit, λ x, by cases x; simp [polycodable.encode]⟩
+
 
 section prod
 
@@ -159,19 +132,68 @@ polycodable.mk'
   (λ x, (decode α (nat.unpair' x).1) >>= (λ x₁, (decode β (nat.unpair' x).2).map $ λ x₂, (x₁, x₂)))
   (λ x, by simp [return, pure])
 begin
-  convert_to is_polytime
-    (λ x, (decode α (nat.unpair' x).1) >>=
-    (λ x₁, (decode β (nat.unpair' x).2).map (
-    λ x₂, nat.mkpair' (encode x₁) (encode x₂)))),
-  { ext x : 1, cases decode α (nat.unpair' x).1; simp, },
-  
+  obtain ⟨somec₁, somep₁, hsome₁⟩ := is_polytime_is_some α,
+  obtain ⟨somec₂, somep₂, hsome₂⟩ := is_polytime_is_some β,
+  obtain ⟨d₁, dp₁, hd₁⟩ := is_polytime_decode α,
+  obtain ⟨d₂, dp₂, hd₂⟩ := is_polytime_decode β,
+  simp only [encode_nat_id] at hd₁ hd₂,
+  obtain ⟨e₁, ep₁, he₁⟩ := is_polytime_encode α,
+  obtain ⟨e₂, ep₂, he₂⟩ := is_polytime_encode β,
+  use (code.ite (somec₁.comp $ d₁.comp code.fst) zero $
+      code.ite (somec₂.comp $ d₂.comp code.snd) zero $ 
+      (code.bit tt).comp (code.pair (tail.comp $ d₁.comp code.fst) (tail.comp $ d₂.comp code.snd))),
+  split,
+  { have P₁ : polytime (d₁.comp code.fst) := polytime_comp dp₁ polytime_fst,
+    have P₂ : polytime (d₂.comp code.snd) := polytime_comp dp₂ polytime_snd,
+    exact (
+      polytime_ite (polytime_comp somep₁ P₁) polytime_zero $
+      polytime_ite (polytime_comp somep₂ P₂) polytime_zero $
+      (polytime_comp (polytime_bit _) (polytime_pair (polytime_comp polytime_tail P₁) (polytime_comp polytime_tail P₂)))), },
+  intro x,
+  cases H₁ : decode α (nat.unpair' x).1, { simp [H₁, hd₁, hsome₁], refl, },
+  cases H₂ : decode β (nat.unpair' x).2, { simp [H₁, hd₁, hsome₁, H₂, hd₂, hsome₂], refl, },
+  simp [H₁, hd₁, hsome₁, H₂, hd₂, hsome₂], simp [polycodable.encode, nat.bit],
 end
 
+lemma polytime_prod_fst (α β : Type) [polycodable α] [polycodable β] : is_polytime (@prod.fst α β) :=
+⟨code.fst, polytime_fst, λ x, by simp [polycodable.encode]⟩
+
+lemma polytime_prod_snd (α β : Type) [polycodable α] [polycodable β] : is_polytime (@prod.snd α β) :=
+⟨code.snd, polytime_snd, λ x, by simp [polycodable.encode]⟩
+
+lemma prod_encode_def (x : α × β) : (encode x.1).mkpair' (encode x.2) = encode x := rfl
 
 end prod
 
--- instance {α β : Type*} [polycodable α] [polycodable β] : polycodable (α × β) :=
--- { encode := λ x, nat.mkpair' (encode x.1) (encode x.2),
---   decode := λ x, decode α (nat.unpair' x).1 >>= (λ x₁, decode β (nat.unpair' x).2 >>= λ x₂, return (x₁, x₂)),
---   decode_encode := _,
---   poly := _ }
+section option
+
+lemma is_polytime_elim {g : α → option β} {f : α × β → γ} {df : α → γ} :
+  is_polytime g → is_polytime f → is_polytime df → is_polytime (λ x, (g x).elim (df x) (λ x', f (x, x')))
+| ⟨gc, gp, hg⟩ ⟨fc, fp, hf⟩ ⟨dfc, dfp, hdf⟩ :=
+⟨code.ite gc dfc (fc.comp $ code.pair code.id (tail.comp gc)), 
+  polytime_ite gp dfp (polytime_comp fp $ polytime_pair polytime_id (polytime_comp polytime_tail gp)),
+  λ x, 
+begin
+  simp only [← prod_encode_def] at hf,
+  cases e : g x with v, { simp [hg, hdf, e, encode], }, { simp [hg, hdf, e, encode, hf (x, v)], }
+end⟩
+
+lemma is_polytime_some : is_polytime (@some α) :=
+⟨code.bit tt, polytime_bit _, by simp [encode, nat.bit]⟩
+
+lemma is_polytime_bind {f : α → option β} {g : α × β → option γ} (hf : is_polytime f) (hg : is_polytime g) :
+  is_polytime (λ x, (f x).bind (λ x', g (x, x'))) :=
+begin
+  convert_to is_polytime (λ x, (f x).elim none (λ x', g (x, x'))),
+  { ext x : 1, cases f x; simp, },
+  exact is_polytime_elim hf hg (is_polytime_const _ none),
+end
+
+lemma is_polytime_map {f : α → option β} {g : α × β → γ} (hf : is_polytime f) (hg : is_polytime g) :
+  is_polytime (λ x, (f x).map (λ x', g (x, x'))) :=
+begin
+  change is_polytime (λ x, (f x).bind (λ x', (some ∘ g) (x, x'))), -- turns out, defeq !
+  exact is_polytime_bind hf (is_polytime_comp is_polytime_some hg),
+end
+
+end option
